src/Semantics/ExprInduction.dfy
@@ -18,167 +18,167 @@ abstract module Ind {
   import opened Equiv
   import opened Utils.Lib.Datatypes
 
-  type {:verify false} Expr = Interp.Expr
+  type Expr = Interp.Expr
 
   //
   // Declarations
   //
 
-  type {:verify false} S(!new)
-  type {:verify false} V(!new)
-  type {:verify false} VS(!new)
+  type S(!new)
+  type V(!new)
+  type VS(!new)
 
   // ``P`` is the property of interest
-  predicate {:verify false} P(st: S, e: Expr)
-  predicate {:verify false} P_Succ(st: S, e: Expr, st': S, v: V) // Success
-  predicate {:verify false} P_Fail(st: S, e: Expr) // Failure
+  predicate P(st: S, e: Expr)
+  predicate P_Succ(st: S, e: Expr, st': S, v: V) // Success
+  predicate P_Fail(st: S, e: Expr) // Failure
 
-  predicate {:verify false} Pes(st: S, es: seq<Expr>)
-  predicate {:verify false} Pes_Succ(st: S, es: seq<Expr>, st': S, vs: VS) // Success
-  predicate {:verify false} Pes_Fail(st: S, es: seq<Expr>) // Failure
+  predicate Pes(st: S, es: seq<Expr>)
+  predicate Pes_Succ(st: S, es: seq<Expr>, st': S, vs: VS) // Success
+  predicate Pes_Fail(st: S, es: seq<Expr>) // Failure
     
-  function {:verify false} AppendValue(v: V, vs: VS): VS // Returns: [v] + vs
-  function {:verify false} SeqVToVS(vs: seq<V>): VS
+  function AppendValue(v: V, vs: VS): VS // Returns: [v] + vs
+  function SeqVToVS(vs: seq<V>): VS
 
-  predicate {:verify false} VS_UpdateStatePre(st: S, vars: seq<string>, argvs: VS)
+  predicate VS_UpdateStatePre(st: S, vars: seq<string>, argvs: VS)
 
   // For the ``Abs`` case
-  function {:verify false} BuildClosureCallState(st: S, vars: seq<string>, body: Expr, env: Environment, argvs: VS): (st':S)
+  function BuildClosureCallState(st: S, vars: seq<string>, body: Expr, env: Environment, argvs: VS): (st':S)
     requires VS_UpdateStatePre(st, vars, argvs)
 
   // For the ``Update`` case
-  function {:verify false} UpdateState(st: S, vars: seq<string>, vals: VS): (st':S)
+  function UpdateState(st: S, vars: seq<string>, vals: VS): (st':S)
     requires VS_UpdateStatePre(st, vars, vals)
 
   // Rollback
-  function {:verify false} StateSaveToRollback(st: S, vars: seq<string>): (st':S)
+  function StateSaveToRollback(st: S, vars: seq<string>): (st':S)
 
-  function {:verify false} StateStartScope(st: S): (st':S)
-  function {:verify false} StateEndScope(st0: S, st: S): (st':S)
+  function StateStartScope(st: S): (st':S)
+  function StateEndScope(st0: S, st: S): (st':S)
 
   // DISCUSS: can't get the postcondition with a constant
-  function {:verify false} GetNilVS(): (vs:VS)
+  function GetNilVS(): (vs:VS)
     ensures vs == SeqVToVS([])
 
-  ghost const {:verify false} NilVS:VS := GetNilVS()
-  ghost const {:verify false} UnitV:V
+  ghost const NilVS:VS := GetNilVS()
+  ghost const UnitV:V
 
-  function {:verify false} VS_Last(vs: VS): V
+  function VS_Last(vs: VS): V
     requires vs != NilVS
 
-  function {:verify false} P_Step(st: S, e: Expr): (res: (S, V))
+  function P_Step(st: S, e: Expr): (res: (S, V))
     requires P(st, e)
     requires !P_Fail(st, e)
     ensures P_Succ(st, e, res.0, res.1)
 
-  function {:verify false} P_StepState(st: S, e: Expr): S
+  function P_StepState(st: S, e: Expr): S
     requires P(st, e)
     requires !P_Fail(st, e)
   {
     P_Step(st, e).0
   }
 
-  function {:verify false} P_StepValue(st: S, e: Expr): V
+  function P_StepValue(st: S, e: Expr): V
     requires P(st, e)
     requires !P_Fail(st, e)
   {
     P_Step(st, e).1
   }
 
-  function {:verify false} Pes_Step(st: S, es: seq<Expr>): (res: (S, VS))
+  function Pes_Step(st: S, es: seq<Expr>): (res: (S, VS))
     requires Pes(st, es)
     requires !Pes_Fail(st, es)
     ensures Pes_Succ(st, es, res.0, res.1)
 
-  function {:verify false} Pes_StepState(st: S, es: seq<Expr>): S
+  function Pes_StepState(st: S, es: seq<Expr>): S
     requires Pes(st, es)
     requires !Pes_Fail(st, es)
   {
     Pes_Step(st, es).0
   }
 
-  function {:verify false} Pes_StepValue(st: S, es: seq<Expr>): VS
+  function Pes_StepValue(st: S, es: seq<Expr>): VS
     requires Pes(st, es)
     requires !Pes_Fail(st, es)
   {
     Pes_Step(st, es).1
   }
 
-  lemma {:verify false} P_Fail_Sound(st: S, e: Expr)
+  lemma P_Fail_Sound(st: S, e: Expr)
     requires P_Fail(st, e)
     ensures P(st, e)
 
-  lemma {:verify false} P_Succ_Sound(st: S, e: Expr, st': S, v: V)
+  lemma P_Succ_Sound(st: S, e: Expr, st': S, v: V)
     requires P_Succ(st, e, st', v)
     ensures P(st, e)
 
-  lemma {:verify false} Pes_Fail_Sound(st: S, es: seq<Expr>)
+  lemma Pes_Fail_Sound(st: S, es: seq<Expr>)
     requires Pes_Fail(st, es)
     ensures Pes(st, es)
 
-  lemma {:verify false} Pes_Succ_Sound(st: S, es: seq<Expr>, st': S, vs: VS)
+  lemma Pes_Succ_Sound(st: S, es: seq<Expr>, st': S, vs: VS)
     requires Pes_Succ(st, es, st', vs)
     ensures Pes(st, es)
 
-  lemma {:verify false} Pes_Succ_Inj(st: S, es: seq<Expr>, st1: S, st1': S, vs: VS, vs': VS)
+  lemma Pes_Succ_Inj(st: S, es: seq<Expr>, st1: S, st1': S, vs: VS, vs': VS)
     requires Pes_Succ(st, es, st1, vs)
     requires Pes_Succ(st, es, st1', vs')
     ensures st1 == st1'
     ensures vs == vs'
 
-  lemma {:verify false} SeqVToVS_Append(v: V, vs: seq<V>)
+  lemma SeqVToVS_Append(v: V, vs: seq<V>)
     ensures AppendValue(v, SeqVToVS(vs)) == SeqVToVS([v] + vs)
 
-  lemma {:verify false} InductVar(st: S, e: Expr)
+  lemma InductVar(st: S, e: Expr)
     requires e.Var?
     requires !P_Fail(st, e)
     ensures P(st, e)
 
-  lemma {:verify false} InductLiteral(st: S, e: Expr)
+  lemma InductLiteral(st: S, e: Expr)
     requires e.Literal?
     ensures P(st, e)
 
-  lemma {:verify false} InductAbs(st: S, e: Expr, vars: seq<string>, body: Expr)
+  lemma InductAbs(st: S, e: Expr, vars: seq<string>, body: Expr)
     requires e.Abs? && e.vars == vars && e.body == body
     requires !P_Fail(st, e)
     requires forall env, argvs | VS_UpdateStatePre(st, vars, argvs) :: P(BuildClosureCallState(st, vars, body, env, argvs), body)
     ensures P(st, e)
 
-  lemma {:verify false} InductAbs_CallState(st: S, e: Expr, vars: seq<string>, body: Expr, env: Environment, argvs: VS, st_ret: S, retv: V)
+  lemma InductAbs_CallState(st: S, e: Expr, vars: seq<string>, body: Expr, env: Environment, argvs: VS, st_ret: S, retv: V)
     requires e.Abs? && e.vars == vars && e.body == body
     requires VS_UpdateStatePre(st, vars, argvs)
     requires !P_Fail(st, e)
     requires P_Succ(BuildClosureCallState(st, vars, body, env, argvs), body, st_ret, retv)
     ensures P(BuildClosureCallState(st, vars, body, env, argvs), body)
 
-  lemma {:verify false} InductExprs_Nil(st: S)
+  lemma InductExprs_Nil(st: S)
     ensures !Pes_Fail(st, []) ==> Pes_Succ(st, [], st, NilVS) // Pes_Fail: because, for instance, the state may not satisfy the proper invariant
 
   // TODO(SMH): I grouped everything (success and failure case) in this lemma. Maybe do the same for some other?...
-  lemma {:verify false} InductExprs_Cons(st: S, e: Expr, es: seq<Expr>)
+  lemma InductExprs_Cons(st: S, e: Expr, es: seq<Expr>)
     ensures P_Fail(st, e) ==> Pes_Fail(st, [e] + es)
     ensures !P_Fail(st, e) ==> forall st1, v :: P_Succ(st, e, st1, v) && Pes_Fail(st1, es) ==> Pes_Fail(st, [e] + es)
     ensures forall st1, v, st2, vs :: P_Succ(st, e, st1, v) && Pes_Succ(st1, es, st2, vs) ==> Pes_Succ(st, [e] + es, st2, AppendValue(v, vs))
 
-  lemma {:verify false} InductApplyLazy_Fail(st: S, e: Expr, arg0: Expr, arg1: Expr)
+  lemma InductApplyLazy_Fail(st: S, e: Expr, arg0: Expr, arg1: Expr)
     requires e.Apply? && e.aop.Lazy? && e.args == [arg0, arg1]
     requires !P_Fail(st, e)
     requires P_Fail(st, arg0)
     ensures P(st, e)
 
-  lemma {:verify false} InductApplyLazy_Succ(st: S, e: Expr, arg0: Expr, arg1: Expr, st1: S, v0: V)
+  lemma InductApplyLazy_Succ(st: S, e: Expr, arg0: Expr, arg1: Expr, st1: S, v0: V)
     requires e.Apply? && e.aop.Lazy? && e.args == [arg0, arg1]
     requires !P_Fail(st, e)
     requires P_Succ(st, arg0, st1, v0)
     requires P(st1, arg1) // We can't assume that we successfully evaluated the second argument, because the operator is lazy
     ensures P(st, e)
 
-  lemma {:verify false} InductApplyEager_Fail(st: S, e: Expr, args: seq<Expr>)
+  lemma InductApplyEager_Fail(st: S, e: Expr, args: seq<Expr>)
     requires e.Apply? && e.aop.Eager? && e.args == args
     requires Pes_Fail(st, args)
     ensures P(st, e)
 
-  lemma {:verify false} InductApplyEagerUnaryOp_Succ(st: S, e: Expr, op: UnaryOps.T, arg0: Expr, st1: S, v0: V)
+  lemma InductApplyEagerUnaryOp_Succ(st: S, e: Expr, op: UnaryOps.T, arg0: Expr, st1: S, v0: V)
     requires e.Apply? && e.aop.Eager? && e.aop.eOp.UnaryOp? && e.aop.eOp.uop == op && e.args == [arg0]
     requires !P_Fail(st, e)
     requires P_Succ(st, arg0, st1, v0)
@@ -187,7 +187,7 @@ abstract module Ind {
     requires Pes_StepValue(st, [arg0]) == SeqVToVS([v0])
     ensures P(st, e)
 
-  lemma {:verify false} InductApplyEagerBinaryOp_Succ(st: S, e: Expr, op: BinaryOps.T, arg0: Expr, arg1: Expr, st1: S, v0: V, st2: S, v1: V)
+  lemma InductApplyEagerBinaryOp_Succ(st: S, e: Expr, op: BinaryOps.T, arg0: Expr, arg1: Expr, st1: S, v0: V, st2: S, v1: V)
     requires e.Apply? && e.aop.Eager? && e.aop.eOp.BinaryOp? && e.aop.eOp.bop == op && e.args == [arg0, arg1]
     requires !P_Fail(st, e)
     requires P_Succ(st, arg0, st1, v0)
@@ -197,7 +197,7 @@ abstract module Ind {
     requires Pes_StepValue(st, [arg0, arg1]) == SeqVToVS([v0, v1])
     ensures P(st, e)
 
-  lemma {:verify false} InductApplyEagerTernaryOp_Succ(
+  lemma InductApplyEagerTernaryOp_Succ(
     st: S, e: Expr, op: TernaryOps.T, arg0: Expr, arg1: Expr, arg2: Expr, st1: S, v0: V, st2: S, v1: V, st3: S, v2: V)
     requires e.Apply? && e.aop.Eager? && e.aop.eOp.TernaryOp? && e.aop.eOp.top == op && e.args == [arg0, arg1, arg2]
     requires !P_Fail(st, e)
@@ -209,13 +209,13 @@ abstract module Ind {
     requires Pes_StepValue(st, [arg0, arg1, arg2]) == SeqVToVS([v0, v1, v2])
     ensures P(st, e)
 
-  lemma {:verify false} InductApplyEagerBuiltinDisplay(st: S, e: Expr, ty: Types.Type, args: seq<Expr>, st1: S, argvs: VS)
+  lemma InductApplyEagerBuiltinDisplay(st: S, e: Expr, ty: Types.Type, args: seq<Expr>, st1: S, argvs: VS)
     requires e.Apply? && e.aop.Eager? && e.aop.eOp.Builtin? && e.aop.eOp.builtin.Display? && e.aop.eOp.builtin.ty == ty && e.args == args
     requires !P_Fail(st, e)
     requires Pes_Succ(st, args, st1, argvs)
     ensures P(st, e)
 
-  lemma {:verify false} InductApplyEagerFunctionCall(st: S, e: Expr, f: Expr, args: seq<Expr>, st1: S, fv: V, st2: S, argvs: VS)
+  lemma InductApplyEagerFunctionCall(st: S, e: Expr, f: Expr, args: seq<Expr>, st1: S, fv: V, st2: S, argvs: VS)
     requires e.Apply? && e.aop.Eager? && e.aop.eOp.FunctionCall? && e.args == [f] + args
     requires !P_Fail(st, e)
     requires P_Succ(st, f, st1, fv)
@@ -225,11 +225,11 @@ abstract module Ind {
     requires Pes_StepValue(st, [f] + args) == AppendValue(fv, argvs)
     ensures P(st, e)
 
-  lemma {:verify false} InductIf_Fail(st: S, e: Expr, cond: Expr, thn: Expr, els: Expr)
+  lemma InductIf_Fail(st: S, e: Expr, cond: Expr, thn: Expr, els: Expr)
     requires e.If? && e.cond == cond && e.thn == thn && e.els == els
     ensures P_Fail(st, cond) ==> P(st, e)
 
-  lemma {:verify false} InductIf_Succ(st: S, e: Expr, cond: Expr, thn: Expr, els: Expr, st_cond: S, condv: V)
+  lemma InductIf_Succ(st: S, e: Expr, cond: Expr, thn: Expr, els: Expr, st_cond: S, condv: V)
     requires e.If? && e.cond == cond && e.thn == thn && e.els == els
     requires !P_Fail(st, e)
     requires P_Succ(st, cond, st_cond, condv)
@@ -237,13 +237,13 @@ abstract module Ind {
     requires P(st_cond, els)
     ensures P(st, e)
 
-  lemma {:verify false} InductUpdate_Fail(st: S, e: Expr, vars: seq<string>, vals: seq<Expr>)
+  lemma InductUpdate_Fail(st: S, e: Expr, vars: seq<string>, vals: seq<Expr>)
     requires e.Update? && e.vars == vars && e.vals == vals
     requires !P_Fail(st, e)
     requires Pes_Fail(st, vals) // Actually, if we have this we have a contradiction - TODO: move to the ensures?
     ensures P(st, e)
 
-  lemma {:verify false} InductUpdate_Succ(
+  lemma InductUpdate_Succ(
     st: S, e: Expr, vars: seq<string>, vals: seq<Expr>, st1: S, values: VS)
     requires e.Update? && e.vars == vars && e.vals == vals
     requires !P_Fail(st, e)
@@ -254,7 +254,7 @@ abstract module Ind {
     ensures P_Succ(st, e, UpdateState(st1, vars, values), UnitV)
     ensures P(st, e)
 
-  lemma {:verify false} InductVarDecl_None_Succ(st: S, e: Expr, vdecls: seq<Exprs.Var>)
+  lemma InductVarDecl_None_Succ(st: S, e: Expr, vdecls: seq<Exprs.Var>)
     requires e.VarDecl? && e.vdecls == vdecls && e.ovals.None?
     requires !P_Fail(st, e)
     // We add this just to make the `StateSaveToRollback` function appear
@@ -263,12 +263,12 @@ abstract module Ind {
       P_Succ(st, e, StateSaveToRollback(st, vars), UnitV)
     ensures P(st, e)
 
-  lemma {:verify false} InductVarDecl_Some_Fail(st: S, e: Expr, vdecls: seq<Exprs.Var>, vals: seq<Expr>)
+  lemma InductVarDecl_Some_Fail(st: S, e: Expr, vdecls: seq<Exprs.Var>, vals: seq<Expr>)
     requires e.VarDecl? && e.vdecls == vdecls && e.ovals.Some? && e.ovals.value == vals
     requires !P_Fail(st, e)
     ensures !Pes_Fail(st, vals)
 
-  lemma {:verify false} InductVarDecl_Some_Succ(st: S, e: Expr, vdecls: seq<Exprs.Var>, vals: seq<Expr>, st1: S, values: VS)
+  lemma InductVarDecl_Some_Succ(st: S, e: Expr, vdecls: seq<Exprs.Var>, vals: seq<Expr>, st1: S, values: VS)
     requires e.VarDecl? && e.vdecls == vdecls && e.ovals.Some? && e.ovals.value == vals
     requires !P_Fail(st, e)
     requires Pes_Succ(st, vals, st1, values)
@@ -284,7 +284,7 @@ abstract module Ind {
       P_Succ(st, e, UpdateState(st2, vars, values), UnitV)
     ensures P(st, e)
 
-  lemma {:verify false} InductBlock_Fail(st: S, e: Expr, stmts: seq<Expr>, st_start: S)
+  lemma InductBlock_Fail(st: S, e: Expr, stmts: seq<Expr>, st_start: S)
     requires e.Block? && e.stmts == stmts
     requires !P_Fail(st, e)
     requires st_start == StateStartScope(st)
@@ -292,7 +292,7 @@ abstract module Ind {
 
   // TODO: make the other lemmas adopt this style, where intermediate values like st_start or vf appear
   // as input parameters
-  lemma {:verify false} InductBlock_Succ(st: S, e: Expr, stmts: seq<Expr>, st_start: S, st_stmts: S, vs: VS, st_end: S, vf: V)
+  lemma InductBlock_Succ(st: S, e: Expr, stmts: seq<Expr>, st_start: S, st_stmts: S, vs: VS, st_end: S, vf: V)
     requires e.Block? && e.stmts == stmts
     requires !P_Fail(st, e)
     requires st_start == StateStartScope(st)
@@ -307,7 +307,7 @@ abstract module Ind {
   // Lemmas
   //
 
-  lemma {:verify false} P_Satisfied(st: S, e: Expr)
+  lemma P_Satisfied(st: S, e: Expr)
     ensures P(st, e)
     decreases e.Size(), 1
   {
@@ -319,7 +319,7 @@ abstract module Ind {
     }
   }
 
-  function {:verify false} InductExprs_Step(st: S, e: Expr, es: seq<Expr>): (out: (S, V, S, VS))
+  function InductExprs_Step(st: S, e: Expr, es: seq<Expr>): (out: (S, V, S, VS))
     requires !Pes_Fail(st, [e] + es)
     ensures
       var (st1, v, st2, vs) := out;
@@ -353,7 +353,7 @@ abstract module Ind {
     (st1, v, st2, vs)
   }
 
-  lemma {:verify false} P_Satisfied_Succ(st: S, e: Expr)
+  lemma P_Satisfied_Succ(st: S, e: Expr)
     requires !P_Fail(st, e)
     ensures P(st, e)
     decreases e.Size(), 0
@@ -566,7 +566,7 @@ abstract module Ind {
     }
   }
 
-  lemma {:verify false} Pes_Satisfied(st: S, es: seq<Expr>)
+  lemma Pes_Satisfied(st: S, es: seq<Expr>)
     ensures Pes(st, es)
     decreases Exprs.Exprs_Size(es), 3
   {
@@ -578,7 +578,7 @@ abstract module Ind {
     }
   }
 
-  lemma {:verify false} Pes_Satisfied_Succ(st: S, es: seq<Expr>)
+  lemma Pes_Satisfied_Succ(st: S, es: seq<Expr>)
     requires !Pes_Fail(st, es)
     ensures Pes(st, es)
     decreases Exprs.Exprs_Size(es), 2
